src/Soundness.v
@@ -1,5 +1,5 @@
 From MCore Require Import Syntax Typing SmallStep Tactics.
-From TLC Require Import LibString LibList.
+From TLC Require Import LibString LibNat LibList LibLogic LibOrder.
 From RecordUpdate Require Import RecordUpdate.
 
 Module Soundness (P : PAT).
@@ -20,22 +20,72 @@ Module Soundness (P : PAT).
       remember empty_env as Gamma eqn:HGamma.
       induction ttype
       ; try (left; constructor).
-      - Case "TmVar". subst. with_hyp (var_in _ _ _) as H. inversion H.
-      - Case "TmApp". right.
+      { Case "TmVar". subst. with_hyp (var_in _ _ _) as H. inversion H. }
+      { Case "TmApp". right.
         forwards* [Hval1 | (t1' & Hstep1)]: IHttype1.
         forwards* [Hval2 | (t2' & Hstep2)]: IHttype2.
-        inverts* Hval1. inverts* ttype1.
-      - Case "TmTyApp". right.
+        inverts* Hval1. inverts* ttype1. }
+      { Case "TmTyApp". right.
         forwards* [Hval | (t' & Hstep)]: IHttype.
-        inverts* Hval. inverts ttype.
+        inverts* Hval. inverts ttype. }
     Qed.
 
-    Lemma tm_subst_gen_preservation :
-      forall vs1 vs2 Gamma t t' ty1 ty2,
-        ok_term (Gamma <| vars := vs1 ++ ty1 :: vs2 |>) t ty2 ->
-        ok_term (Gamma <| vars := vs1 ++ vs2 |>) t' ty1 ->
-        ok_term (Gamma <| vars := vs1 ++ vs2 |>) (tm_subst_gen t (length vs1) t') ty2.
+    Lemma ok_kind_ignores_vars :
+      forall Gamma vs k,
+        ok_kind Gamma k ->
+        ok_kind (Gamma <| vars := vs |>) k.
     Proof. Admitted.
+
+    Lemma ok_type_ignores_vars :
+      forall Gamma vs ty k,
+        ok_type Gamma ty k ->
+        ok_type (Gamma <| vars := vs |>) ty k.
+    Proof. Admitted.
+
+    Lemma ok_term_tvars_weaken :
+      forall Gamma k t ty,
+        ok_term Gamma t ty ->
+        ok_term (Gamma <| tvars ::= fun tvs => k :: tvs |>) (tm_ty_shift t) ty.
+    Proof. Admitted.
+
+    Lemma ok_term_vars_weaken :
+      forall Gamma ty' t ty,
+        ok_term Gamma t ty ->
+        ok_term (Gamma <| vars ::= fun vs => ty' :: vs |>) (tm_shift t) ty.
+    Proof. Admitted.
+
+    Lemma tm_subst_gen_preservation :
+      forall vs1 vs2 tvs Gamma t t' ty1 ty2,
+        ok_term (Gamma <| vars := vs1 ++ ty1 :: vs2 |> <| tvars := tvs |>) t ty2 ->
+        ok_term (Gamma <| vars := vs1 ++ vs2 |> <| tvars := tvs |>) t' ty1 ->
+        ok_term (Gamma <| vars := vs1 ++ vs2 |> <| tvars := tvs |>) (tm_subst_gen t (length vs1) t') ty2.
+    Proof.
+      introv ttype ttype'.
+      remember (Gamma <| vars := vs1 ++ ty1 :: vs2 |> <| tvars := tvs |>) as Gamma' eqn:HGamma.
+      gen t' vs1 tvs.
+      induction* ttype ; intros ; subst.
+      { Case "TmVar". with_hyp (var_in _ _ _) as Hvar. unfold tm_subst_gen.
+        lets [ in_vs1 | (m & Heqm & in_vs2') ] : Nth_app_inv Hvar.
+        { lets Hlt : Nth_inbound in_vs1. rewrites (>> If_l Hlt).
+          constructor. applys* Nth_app_l. }
+        { subst. assert (nlt : ~(length vs1 + m < length vs1)). nat_math.
+          rewrites (>> If_r nlt).
+          lets [ (Heq0 & Heq) | (m' & Heqm' & in_vs2) ] : Nth_cons_inv in_vs2' ; subst.
+          { rewrites* (>> If_l plus_zero_r). }
+          { rew_nat. assert (neq : ~(S (length vs1 + m') = length vs1)). nat_math.
+            rewrites (>> If_r neq). rewrite Nat.add_comm.
+            constructor. applys Nth_app_r in_vs2. } } }
+      { Case "TmLam". constructors*.
+        applys* ok_type_ignores_vars (Gamma <| vars := vs1 ++ ty1 :: vs2 |> <| tvars := tvs |>).
+        folds (tm_subst_gen t (S (length vs1)) (tm_shift t')).
+        applys* IHttype (tm_shift t') (ty0 :: vs1).
+        applys_eq* (ok_term_vars_weaken (Gamma <| vars := vs1 ++ vs2 |> <| tvars := tvs |>) ty0). }
+      { Case "TmTyLam". constructors*.
+        applys* ok_kind_ignores_vars (Gamma <| vars := vs1 ++ ty1 :: vs2 |> <| tvars := tvs |>).
+        applys* IHttype. applys* ok_term_tvars_weaken (Gamma <| vars := vs1 ++ vs2 |> <| tvars := tvs |>). }
+      { Case "TmTyApp". constructors*.
+        applys* ok_type_ignores_vars (Gamma <| vars := vs1 ++ ty1 :: vs2 |> <| tvars := tvs |>). }
+    Qed.
 
     Lemma tm_subst_preservation :
       forall Gamma t t' ty1 ty2,
@@ -43,7 +93,8 @@ Module Soundness (P : PAT).
         ok_term Gamma t' ty1 ->
         ok_term Gamma (tm_subst t t') ty2.
     Proof.
-      intros. applys_eq (tm_subst_gen_preservation nil Gamma.(vars) Gamma t t' ty1) ; destruct* Gamma.
+      intros. applys_eq* (tm_subst_gen_preservation nil Gamma.(vars) Gamma.(tvars) Gamma t t' ty1) ;
+        destruct* Gamma.
     Qed.
 
     Lemma tm_ty_subst_preservation :
@@ -64,8 +115,8 @@ Module Soundness (P : PAT).
       induction ttype ; intros ; inverts tstep
       ; try (with_hyp (is_context _) as ctx ; with_hyp (_ = _) as eq
              ; inverts ctx ; inverts* eq).
-      - Case "TmApp". inverts ttype1. applys* tm_subst_preservation.
-      - Case "TmTyApp". inverts ttype. applys* tm_ty_subst_preservation.
+      { Case "TmApp". inverts ttype1. applys* tm_subst_preservation. }
+      { Case "TmTyApp". inverts ttype. applys* tm_ty_subst_preservation. }
     Qed.
   End Soundness.
 End Soundness.
